a little more OOp

Oop.v
@@ -7,6 +7,7 @@ between variables x , y, . . . , e.g., the formal parameters of methods, includi
  I am less interested in OOP and more in trace semantics*)
 
 From Coq Require Import Strings.String.
+Open Scope string_scope.
 From Coq Require Import Bool.Bool.
 From Coq Require Import Arith.EqNat. Import Nat.
 From Coq Require Import Init.Datatypes.
@@ -14,9 +15,6 @@ From Coq Require Import Lists.List.
 Import ListNotations.
 From Coq Require Import Program.   (* for `dependent induction` *)
 From Coq Require Import Relations.
-
-From SymEx Require Import Expr.
-From SymEx Require Import Maps.
 
 Inductive Oexpr : Type :=
 | PNil
@@ -33,7 +31,9 @@ with  Bexpr  :=
 | BAnd (b1 b2:Bexpr)
 | BEq (e1 e2:Oexpr).
 
-Definition r : Oexpr := PVar (HVar "r").
+Coercion PVar : Heap >-> Oexpr.
+
+Definition r : Heap := HVar "r".
 
 Inductive Stmt : Type :=
 | SAsgn (h:Heap) (e:Oexpr)
@@ -47,8 +47,12 @@ Inductive Stmt : Type :=
   (*just one method with no parameters per class for now*)
   | CDec (body:Stmt).
 
-Open Scope com_scope.
+Declare Custom Entry com.
+Declare Scope com_scope.
 
+Notation "<{ e }>" := e (at level 0, e custom com at level 99) : com_scope.
+Notation "( x )" := x (in custom com, x at level 99) : com_scope.
+Notation "x" := x (in custom com at level 0, x constr at level 0) : com_scope.
 Notation "x '==' y" := (BEq x y)
             (in custom com at level 0, x constr at level 0,
              y at level 85, no associativity) : com_scope.
@@ -88,6 +92,8 @@ Notation "'class' '{' b '}'"  :=
             (in custom com at level 0,
                 b at level 85, no associativity) : com_scope.
 
+Open Scope com_scope.
+
 Fixpoint Oexpr_subst (e e0:Oexpr) : Oexpr :=
   match e with
   | PNil => PNil
@@ -105,7 +111,7 @@ Fixpoint Oexpr_subst (e e0:Oexpr) : Oexpr :=
   | BEq e1 e2 => BEq (Oexpr_subst e1 e0) (Oexpr_subst e2 e0)
   end.
 
-Fixpoint Heap_subst (h:Heap) (e0:Oexpr) : Heap :=
+Definition Heap_subst (h:Heap) (e0:Oexpr) : Heap :=
   match h with
   | HVar x => HVar x
   | HExpr e f => HExpr (Oexpr_subst e e0) f
@@ -128,8 +134,7 @@ Definition pc : Bexpr -> TraceStep :=
   fun b => inl (inl b).
 Definition new : (Heap * Class) -> TraceStep :=
   fun x => inl (inr x).
-Definition asgn : (Heap * Oexpr) -> TraceStep :=
-  fun x => inr x.
+Definition asgn : (Heap * Oexpr) -> TraceStep := inr.
 
 Open Scope list_scope.
 Definition Trace : Type := list TraceStep.
@@ -140,14 +145,226 @@ Reserved Notation " c '->s' c' " (at level 40).
 
 Inductive Sstep : relation SState :=
 | SAsgn_step : forall h e s p,
-    (<{ h := e ; s }>, p) ->s (s, asgn (h, e) :: p)
+    (<{ h := e ; s }>, p) ->s (s, p ++ [asgn (h, e)])
 | SNew_step : forall h C s p x,
     (*maybe an "x fresh" condition here*)
-    (<{ h := new C ; s }>, p) ->s (s, asgn (h, PVar x) :: new (x, C) :: p)
+    (<{ h := new C ; s }>, p) ->s (s, p ++ [ asgn (h, PVar x) ; new (x, C)])
 | SMethod_step : forall h e0 s s' p,
     (<{ h <- class { s } (e0) ; s'}>, p)
-    ->s (SSeq (method_subst s e0) <{ h := r ; s'}>, pc (BNot (BEq e0 PNil)):: p)
+    ->s (SSeq (method_subst s e0) <{ h := r ; s'}>, p ++ [pc (BNot (BEq e0 PNil))])
+| SReturn_step : forall e s p,
+    (<{ return e ; s }>, p) ->s (s, p ++ [asgn (r, e)])
+| SIfTrue_step : forall b s1 s2 s p,
+    (<{ if b {s1}{s2} ; s}>, p) ->s (<{ s1 ; s }>, p ++ [pc b])
+| SIfFalse_step : forall b s1 s2 s p,
+    (<{ if b {s1}{s2} ; s}>, p) ->s (<{ s2 ; s }>, p ++ [pc (BNot b)])
+| SWhileTrue_step : forall b s s' p,
+    (<{ while b {s} ; s' }>, p) ->s (<{ s ; while b {s} ; s' }>, p ++ [pc b])
+| SWhileFalse_step : forall b s s' p,
+    (<{ while b {s} ; s' }>, p) ->s (s', p ++ [pc (BNot b)])
   where " c '->s' c' " := (Sstep c c').
 
 Definition multi_Sstep := clos_refl_trans_n1 _ Sstep.
 Notation " c '->*' c' " := (multi_Sstep c c') (at level 40).
+
+Fixpoint subst_expr (e': Oexpr) (x:string) (e:Oexpr) : Oexpr :=
+  match e' with
+  | PVar (HExpr e0 f) => PVar (HExpr (subst_expr e0 x e) f)
+  | HVar y => if (x =? y)%string then e else HVar y
+  | PCond b e1 e2 => PCond (subst_bexpr b x e) (subst_expr e1 x e) (subst_expr e2 x e)
+  | e' => e'
+  end
+with subst_bexpr (b:Bexpr) (x:string) (e:Oexpr) : Bexpr :=
+       match b with
+       | BNot b => BNot (subst_bexpr b x e)
+       | BAnd b1 b2 => BAnd (subst_bexpr b1 x e) (subst_bexpr b2 x e)
+       | BEq e1 e2 => BEq (subst_expr e1 x e) (subst_expr e2 x e)
+       | b => b
+       end.
+
+Fixpoint subst_heap (e': Oexpr) (h:Oexpr) (f:string) (e:Oexpr) : Oexpr :=
+  match e' with
+  | PVar (HExpr e0 f') => if (f =? f')%string
+                         then PCond (BEq (subst_heap e0 h f e) h) e (subst_heap e0 h f e)
+                         else PVar (HExpr (subst_heap e0 h f e) f')
+  | PCond b e1 e2 => PCond (subst_bexpr_heap b h f e) (subst_heap e1 h f e) (subst_heap e2 h f e)
+  | e' => e'
+  end
+with subst_bexpr_heap (b:Bexpr) (h:Oexpr) (f:string) (e:Oexpr) : Bexpr :=
+       match b with
+       | BNot b => BNot (subst_bexpr_heap b h f e)
+       | BAnd b1 b2 => BAnd (subst_bexpr_heap b1 h f e) (subst_bexpr_heap b2 h f e)
+       | BEq e1 e2 => BEq (subst_heap e1 h f e) (subst_heap e2 h f e)
+       | b => b
+       end.
+
+(* the article includes a class here, but then never use it? *)
+Fixpoint subst_newB (b:Bexpr) (x:string) : Bexpr :=
+  match b with
+  | BNot b => BNot (subst_newB b x)
+  | BAnd b1 b2 => BAnd (subst_newB b1 x) (subst_newB b2 x)
+  | BEq (HVar y) (HVar z) => if (y =? x)%string && (z =? x)%string then BTrue else BFalse
+  | BEq _ _ => BFalse
+  | b => b
+  end.
+
+Fixpoint subst_newHB (b:Bexpr) (h:Oexpr) (f:string) : Bexpr :=
+  match b with
+  | BNot b => BNot (subst_newHB b h f)
+  | BAnd b1 b2 => BAnd (subst_newHB b1 h f) (subst_newHB b2 h f)
+  | BEq _ _ => BFalse
+  | b => b
+  end.
+
+Fixpoint subst_new (e: Oexpr) (x:string) : Oexpr :=
+  match e with
+  | PNil => PNil
+  | PThis => PThis
+  | HVar y => HVar y
+  | HExpr (HVar y) f => if (x =? y)%string then PNil else HExpr (HVar y) f
+  | HExpr e f => HExpr (subst_new e x) f
+  | PCond b e1 e2 => PCond (subst_newB b x) (subst_new e1 x) (subst_new e2 x)
+  end.
+
+Fixpoint nil_error_absence (e:Oexpr) : Bexpr :=
+  match e with
+  | PVar (HExpr e f) =>  BAnd <{ ~ (e == nil) }> (nil_error_absence e)
+  | PCond b e1 e2 => BAnd (nil_error_absenceB b) (BAnd (nil_error_absence e1) (nil_error_absence e2))
+  | _ => BTrue
+  end
+with nil_error_absenceB (b:Bexpr) : Bexpr :=
+       match b with
+       | BNot b => nil_error_absenceB b
+       | BAnd b1 b2 => BAnd (nil_error_absenceB b1) (nil_error_absenceB b2)
+       | BEq e1 e2 => BAnd (nil_error_absence e1) (nil_error_absence e2)
+       | _ => BTrue
+       end.
+
+Fixpoint path_condition (t:Trace) : Bexpr :=
+  match t with
+  | [] => BTrue
+  | inl (inl b) :: p => BAnd (path_condition p) b
+  | inl (inr (HVar x, C)) :: p => subst_newB (path_condition p) x
+  | inl (inr (HExpr h f, C)) :: p => subst_newHB (path_condition p) h f
+  | inr (HVar x, e) :: p => BAnd (subst_bexpr (path_condition p) x e) (nil_error_absence e)
+  | inr (HExpr h f, e) :: p => BAnd (subst_bexpr_heap (path_condition p) h f e)
+                               (BAnd (nil_error_absence h) (nil_error_absence e))
+  end.
+
+(** Concrete Semantics *)
+
+(* we "cheat" by just evaluating to symbols represented by strings *)
+Definition Obs : Type := string.
+Definition Val : Type := string.
+
+Definition GVal : Type := string -> Obs.
+Definition HVal : Type := Obs -> string -> Val.
+
+Fixpoint eval (G:GVal) (H:HVal) (e:Oexpr) : option Val :=
+  match e with
+  | PNil => Some "nil"
+  | PThis => Some "this"
+  | HVar x => Some (G x)
+  | PVar (HExpr e f) => match eval G H e with
+                       | None => None
+                       | Some o => if f =? "nil" then None else
+                           if o =? "nil" then None else Some (H o f)
+                       end
+  | PCond b e1 e2 => match evalB G H b with
+                      | None => None
+                    | Some true => eval G H e1
+                    | Some false => eval G H e2
+                    end
+                      end
+  with evalB (G:GVal) (H:HVal) (b:Bexpr) : option bool:=
+         match b with
+         | BTrue => Some true
+         | BFalse => Some false
+         | BNot b => option_map negb (evalB G H b)
+         | BAnd b1 b2 => match evalB G H b1 with
+                        | None => None
+                        | Some b1 => option_map (andb b1) (evalB G H b2)
+                        end
+         | BEq e1 e2 => match eval G H e1 with
+                       | None => None
+                       | Some o1 => match eval G H e2 with
+                                   | None => None
+                                   | Some o2 => Some (o1 =? o2)
+                                   end
+                       end
+         end.
+
+Definition update {E:Type} (s: string -> E) (x:string) (e:E) : string -> E :=
+  fun y => if String.eqb x y then e else s x.
+
+Definition CConfig : Type := GVal * HVal * Trace.
+
+Reserved Notation " c '=>c' c' " (at level 40).
+
+Definition Hupdate (H:HVal) (o:Obs) (f:string) (v:Val) : HVal :=
+  fun (o':Obs) (f':string) => if (o =? o') && (f =? f') then v else H o' f'.
+
+Inductive Cstep : relation CConfig :=
+| CHAsgn_step : forall G H h h' f e e' p,
+    eval G H h = Some h' ->
+    eval G H e = Some e' ->
+    (G, H, asgn (HExpr h f,e) :: p) =>c (G , Hupdate H h' f e', p)
+| CGAsgn_step : forall G H x e e' p,
+    eval G H e = Some e' ->
+    (G, H, asgn (HVar x, e) :: p) =>c (update G x e', H, p)
+| CGNew_step : forall G H x f C p o,
+    (* o fresh? *)
+    (G, H, new (HVar x, C) :: p) =>c (update G x o, Hupdate H o f "nil", p)
+(* this means new objects cannot be assigned to fields, which is maybe non intentional *)
+| CTest_step : forall G H b p,
+    evalB G H b = Some true ->
+    (G, H, pc b :: p) =>c (G, H, p)
+  where " c '=>c' c' " := (Cstep c c').
+
+Definition multi_Cstep := clos_refl_trans_1n _ Cstep.
+Notation " c '=>*' c' " := (multi_Cstep c c') (at level 40).
+
+Definition computes (G:GVal) (H:HVal) (p:Trace) : Prop := exists G' H', (G, H, p) =>* (G', H', []).
+
+Lemma some_not_none {T:Type} (x:T) : Some x <> None.
+Proof. intro. inversion H. Qed.
+
+Lemma none_not_some {T:Type} (x:T) : None <> Some x.
+Proof. intro. inversion H. Qed.
+
+Lemma some_injective {T:Type} (x y:T) : Some x = Some y -> x = y.
+Proof. intros. inversion H. reflexivity. Qed.
+
+Theorem sound_and_complete : forall G H p,
+    computes G H p <-> evalB G H (path_condition p) = Some true.
+Proof.
+  intros. induction p.
+  - split; intro.
+    + reflexivity.
+    + exists G. exists H. constructor.
+  - destruct a as [[b | (h, C)] | x].
+    (* boolean test *)
+    + split; intro.
+      * destruct H0 as [G' [H' comp]]. destruct IHp as [IHright IHleft].
+        inversion comp; subst.
+        inversion H0; subst.
+        simpl. rewrite IHright. rewrite H8. reflexivity.
+        exists G'. exists H'. apply H1.
+      * destruct IHp as [IHright IHleft].
+        inversion H0; subst. destruct (evalB G H (path_condition p)). destruct b0.
+        ** destruct (IHleft eq_refl) as [G' [H' c]].
+        exists G'. exists H'. econstructor.
+           *** apply CTest_step. destruct (evalB G H b).
+               inversion H2. reflexivity.
+               simpl in H2. apply none_not_some in H2. contradiction.
+           *** assumption.
+        ** destruct (evalB G H b); try destruct b0;
+             simpl in H2; try (apply some_injective in H2); discriminate.
+        ** discriminate.
+    (* new *)
+    + admit. (* needs a C-aware substB, which I haven't figured out *)
+      + split; intro.
+        ++ destruct H0 as [G' [H' comp]]. destruct IHp as [IHright IHleft].
+           inversion comp; subst.
+           inversion H0; subst.
+           * simpl.
